# problems:
# the ontology is missing an sdo:license property and has two provenance properties, dcterms:source and dcterms:provenance defined
# abisdm:conservationStatus is missing a definintion and an isDefinedBy property

# baseURI: https://linked.data.gov.au/def/abisdm

@prefix dcat: <http://www.w3.org/ns/dcat#> .
@prefix dcterms: <http://purl.org/dc/terms/> .
@prefix ex: <http://example.com/thing/> .
@prefix abisdm: <https://linked.data.gov.au/def/abisdm/> .
@prefix owl: <http://www.w3.org/2002/07/owl#> .
@prefix prov: <http://www.w3.org/ns/prov#> .
@prefix rdf: <http://www.w3.org/1999/02/22-rdf-syntax-ns#> .
@prefix rdfs: <http://www.w3.org/2000/01/rdf-schema#> .
@prefix skos: <http://www.w3.org/2004/02/skos/core#> .
@prefix sdo: <https://schema.org/> .
@prefix sosa: <http://www.w3.org/ns/sosa/> .
@prefix tern: <https://w3id.org/tern/ontologies/tern/> .
@prefix time: <http://www.w3.org/2006/time#> .
@prefix void: <http://rdfs.org/ns/void#> .
@prefix xsd: <http://www.w3.org/2001/XMLSchema#> .


<https://linked.data.gov.au/def/abisdm>
  a owl:Ontology ;
  skos:prefLabel "ABIS Data Management Ontology"@en ;
  skos:definition """An ontology containing elements for data management for Australian Biodiversity Information Standard (ABIS) data. 
  
This ontology is not a domain model for ABIS - that is the TERN Ontology (https://w3id.org/tern/ontologies/tern/). This ontology provides non-scientific model elements for data management, such as properties to indicate whether species are endangered or not, data publication embargo periods and so on."""@en ;
  sdo:creator <https://linked.data.gov.au/org/dawe> ;
  sdo:publisher <https://linked.data.gov.au/org/dawe> ;
  sdo:dateCreated "2022-03-22"^^xsd:date ;
  sdo:dateModified "2022-04-02"^^xsd:date ;
  sdo:dateIssued "2022-03-22"^^xsd:date ;
  # sdo:license "https://creativecommons.org/licenses/by/4.0/"^^xsd:anyURI ;
  sdo:copyrightHolder <https://linked.data.gov.au/org/dawe> ;
  sdo:copyrightNotice "(c) Commonwealth of Australia (Department of Agriculture, Water and the Environment), 2022" ;
  dcterms:provenance "This ontology has been made as part of the BDR Pilot project work"@en ;
  dcterms:source "http://example.com/fake-source"^^xsd:anyURI ;
  owl:versionIRI <https://linked.data.gov.au/def/abisdm/0.1.1> ;
  owl:versionInfo "0.1.0" ;
  sdo:codeRespository "https://bdr.gov.au"^^xsd:anyURI ;
.

<https://linked.data.gov.au/org/dawe>
  a sdo:Organization ;
  sdo:name "Department of Agriculture, Water and the Environment"@en ;
  sdo:url "https://www.awe.gov.au"^^xsd:anyURI ;
.

abisdm:SuperClass
    a owl:Class , rdfs:Class ;
    rdfs:subClassOf owl:Thing ;
    skos:prefLabel "ABIS DM Ontology Superclass" ;
    skos:definition "A superclass of the main things in the ABIS DB Ontology" ;
    rdfs:isDefinedBy <https://linked.data.gov.au/def/abisdm> ;
    dcterms:provenance "Created for the Bidiversity Data Repository project. It is required for good data display within the BDR technical system."@en ;
    skos:example """This class is not expected to be instantiated"""@en ;
.

abisdm:ConservationStatus
  a owl:Class ;
  rdfs:subClassOf abisdm:SuperClass , skos:Concept ;
  skos:definition "A code indicating the conservation status of a taxon or a proxy object for a taxon, such as a taxon name"@en ;
  skos:prefLabel "Created for the Bidiversity Data Repository project. Conservation Status"@en ;
  dcterms:provenance "Motivated by the existence of multiple conservation status code lists" ;
  rdfs:isDefinedBy <https://linked.data.gov.au/def/abisdm> ;
  skos:example """# instances of this class are stored as Concepts in the Conservation Status vocabulary 
# https://linked.data.gov.au/def/conservation-statuses, e.g.
<https://linked.data.gov.au/def/conservation-statuses/CR> 
    a skos:Concept , abisdm:ConservationStatus ;
    skos:prefLabel "Critically Endangered" ;
.""" ;
.

abisdm:conservationStatus
  a owl:ObjectProperty ;  
  # skos:definition "Indicates a Conservation Status"@en ;
  skos:prefLabel "conservation status"@en ;
  dcterms:provenance "Created for the Bidiversity Data Repository project. Motivated by the existence of multiple conservation status code lists" ;
  # rdfs:isDefinedBy <https://linked.data.gov.au/def/abisdm> ;
  sdo:rangeIncludes tern:Taxon ;
  rdfs:range abisdm:ConservationStatus ;
  skos:example """# the example taxon, :Calothamnus-lateralis-var-crassus, is indicated as Critically Endangered, cstat:CR
# using a Concept from the the Conservation Status vocabulary
@prefix ex: <http://example.com/> .
@prefix cstat: <https://linked.data.gov.au/def/conservation-statuses/> .

ex:Calothamnus-lateralis-var-crassus abisdm:conservationStatus cstat:CR .""" ;
.

abisdm:embargoEndDate
  a owl:DatatypeProperty ;
  skos:prefLabel "embargo end date"@en ;
  skos:definition """The date after which the emabrgo on this Dataset no longer applies.
  
This property takes precedence over abisdm:embargoPeriod if both are present."""@en ;
  rdfs:range xsd:date ;
  dcterms:provenance "Created for the Bidiversity Data Repository project" ;
  rdfs:isDefinedBy <https://linked.data.gov.au/def/abisdm> ;
  skos:example """# Dataset with a fixed embargo end date
@prefix abisdm: <https://linked.data.gov.au/def/abisdm/> .
@prefix dcterms: <http://purl.org/dc/terms/> .
@prefix sdo: <https://schema.org/> .
@prefix tern: <https://w3id.org/tern/ontologies/tern/> .
@prefix xsd: <http://www.w3.org/2001/XMLSchema#> .

<http://example.org/dataset/embargoed-test-01>
    a tern:RDFDataset ;
    dcterms:title "Margaret River Flora" ;
    skos:definition "202201 CBR Flora and Vegetation report_draftv1.pdf by Stream Environment and Water Pty Ltd" ;
    dcterms:creator <http://example.org/Stream-Environment-and-Water-Pty-Ltd> ;
    dcterms:created "2022-02-24"^^xsd:date ;
    abisdm:embargoEndDate "2022-08-15"^^xsd:date ;
.

<http://example.org/Stream-Environment-and-Water-Pty-Ltd>
    a sdo:Organization ;
    sdo:name "Stream Environment and Water Pty Ltd" ;
.""" ;
.

abisdm:embargoPeriod
  a owl:DatatypeProperty ;
  skos:prefLabel "embargo period"@en ;
  skos:definition "The period of time for which this Dataset is embargoed. The time's start date must be set by the system embargoing the data. It may be calculated from a dataset creation/issued date but, if those properties are missing, should be calculated from the date at which the embargoing system recieved the Dataset."@en ;  
  rdfs:range xsd:duration ;
  rdfs:isDefinedBy <https://linked.data.gov.au/def/abisdm> ;
  dcterms:provenance "Created for the Bidiversity Data Repository project" ;
  skos:example """# Dataset with a embargo period
@prefix abisdm: <https://linked.data.gov.au/def/abisdm/> .
@prefix dcterms: <http://purl.org/dc/terms/> .
@prefix sdo: <https://schema.org/> .
@prefix tern: <https://w3id.org/tern/ontologies/tern/> .
@prefix xsd: <http://www.w3.org/2001/XMLSchema#> .

<http://example.org/dataset/embargoed-test-01>
    a tern:RDFDataset ;
    dcterms:title "Margaret River Flora" ;
    skos:definition "202201 CBR Flora and Vegetation report_draftv1.pdf by Stream Environment and Water Pty Ltd" ;
    dcterms:creator <http://example.org/Stream-Environment-and-Water-Pty-Ltd> ;
    dcterms:created "2022-02-24"^^xsd:date ;
    abisdm:embargoPeriod "P1Y6M"^^xsd:duration ;
.

<http://example.org/Stream-Environment-and-Water-Pty-Ltd>
    a sdo:Organization ;
    sdo:name "Stream Environment and Water Pty Ltd" ;
.""" ;
.

